Bytestring/BitVec.lean
@@ -1,0 +1,89 @@
+namespace BitVec
+
+def ult' (b b' : BitVec w) : Bool :=
+  match w with
+  | 0 => false
+  | w' + 1 =>
+    match b.msb, b'.msb with
+    | false, true => true
+    | true, false => false
+    | false, false => ult' (b.setWidth w') (b'.setWidth w')
+    | true, true => ult' (b.setWidth w') (b'.setWidth w')
+
+theorem ult_zero_length {b b' : BitVec 0} : b.ult b' = false := by
+  simp [BitVec.ult, BitVec.toNat_zero_length]
+
+theorem toNat_div_two_pow {b : BitVec (w + 1)} : b.toNat / 2 ^ w = if b.msb then 1 else 0 := by
+  apply Nat.eq_of_testBit_eq
+  intro i
+  rw [Nat.testBit_div_two_pow]
+  cases i with
+  | zero =>
+    rw [Nat.zero_add, testBit_toNat, BitVec.msb_eq_getLsbD_last,
+      Nat.add_sub_cancel]
+    split <;> simp_all
+  | succ i =>
+    rw [testBit_toNat, getLsbD_of_ge _ _ (by omega)]
+    split <;> simp [← Bool.not_eq_true, Nat.testBit_one_eq_true_iff_self_eq_zero]
+
+theorem ult'_eq_ult {b b' : BitVec w} : ult' b b' = BitVec.ult b b' := by
+  fun_induction ult' with
+  | case1 => simp [ult_zero_length]
+  | case2 w' b b' h₁ h₂ => simp_all [ult_eq_msb_of_msb_neq]
+  | case3 => simp_all [ult_eq_msb_of_msb_neq]
+  | case4 w' b b' h₁ h₂ ih  =>
+    rw [ih, ult_eq_decide, ult_eq_decide, decide_eq_decide, toNat_setWidth,
+      toNat_setWidth]
+    conv => rhs; rw [← Nat.div_add_mod b.toNat (2 ^ w'), ← Nat.div_add_mod b'.toNat (2 ^ w')]
+    simp [toNat_div_two_pow, h₁, h₂]
+  | case5 w' b b' h₁ h₂ ih =>
+    rw [ih, ult_eq_decide, ult_eq_decide, decide_eq_decide, toNat_setWidth,
+      toNat_setWidth]
+    conv => rhs; rw [← Nat.div_add_mod b.toNat (2 ^ w'), ← Nat.div_add_mod b'.toNat (2 ^ w')]
+    simp [toNat_div_two_pow, h₁, h₂]
+
+set_option grind.warning false
+
+theorem lt_iff_getElem {b b' : BitVec w} :
+    b < b' ↔ ∃ (i : Nat) (h : i < w), b[i] = false ∧ b'[i] = true ∧ ∀ j, i < j → (_ : j < w) → b[j] = b'[j] := by
+  rw [← ult_iff_lt, ← ult'_eq_ult]
+  fun_induction ult' with
+  | case1 => simp
+  | case2 w' b b' h₁ h₂ =>
+    simp only [Nat.succ_eq_add_one, true_iff]
+    refine ⟨w', by omega, ?_, ?_, by omega⟩
+    · rw [msb_eq_getLsbD_last, Nat.add_sub_cancel] at h₁
+      rwa [← getLsbD_eq_getElem]
+    · rw [msb_eq_getLsbD_last, Nat.add_sub_cancel] at h₂
+      rwa [← getLsbD_eq_getElem]
+  | case3 w' b b' h₁ h₂ =>
+    simp only [Bool.false_eq_true, Nat.succ_eq_add_one, false_iff, not_exists, _root_.not_and,
+      Classical.not_forall, not_imp]
+    intro j hj hj₁ hj₂
+    rw [msb_eq_getLsbD_last, Nat.add_sub_cancel] at h₁ h₂
+    rw [← getLsbD_eq_getElem] at hj₁ hj₂
+    refine ⟨w', ?_, by omega, ?_⟩
+    · exact Or.elim (by omega : j < w' ∨ j = w') id (by rintro rfl; simp_all)
+    · simp [← getLsbD_eq_getElem, h₁, h₂]
+  | case4 w' b b' h₁ h₂ ih =>
+    rw [msb_eq_getLsbD_last, Nat.add_sub_cancel] at h₁ h₂
+    simp only [ih, ← getLsbD_eq_getElem, getLsbD_setWidth, Bool.and_eq_false_imp, decide_eq_true_eq,
+      Bool.and_eq_true, exists_and_left, exists_prop, Nat.succ_eq_add_one]
+    refine ⟨fun ⟨i, hi⟩ => ⟨i, by grind, by grind, by grind, ?_⟩,
+      fun ⟨i, hi⟩ => ⟨i, by grind, by grind, by grind, ?_⟩⟩
+    · exact fun j hj hjw' => Or.elim (by omega : j = w' ∨ j < w') (by grind) (by grind)
+    · refine fun j hj hjw' => ?_
+      simp only [hjw', decide_true, Bool.true_and]
+      exact hi.2.2.2 _ hj (by omega)
+  | case5 w' b b' h₁ h₂ ih =>
+    rw [msb_eq_getLsbD_last, Nat.add_sub_cancel] at h₁ h₂
+    simp only [ih, ← getLsbD_eq_getElem, getLsbD_setWidth, Bool.and_eq_false_imp, decide_eq_true_eq,
+      Bool.and_eq_true, exists_and_left, exists_prop, Nat.succ_eq_add_one]
+    refine ⟨fun ⟨i, hi⟩ => ⟨i, by grind, by grind, by grind, ?_⟩,
+      fun ⟨i, hi⟩ => ⟨i, by grind, by grind, by grind, ?_⟩⟩
+    · exact fun j hj hjw' => Or.elim (by omega : j = w' ∨ j < w') (by grind) (by grind)
+    · refine fun j hj hjw' => ?_
+      simp only [hjw', decide_true, Bool.true_and]
+      exact hi.2.2.2 _ hj (by omega)
+
+end BitVec
